ocaml/fstar-tests/generated/FStar_Tests_Pars.ml
@@ -759,32 +759,36 @@ let (parse_incremental_decls : unit -> unit) =
     | uu___2 ->
         FStar_Compiler_Effect.failwith
           "Incremental parsing failed: Unexpected output"
-let (parse_somelang :
-  Prims.string ->
-    FStar_Compiler_Range_Type.range ->
-      (FStar_Parser_AST_Util.error_message, FStar_Parser_AST.decl Prims.list)
-        FStar_Pervasives.either)
+let parse_somelang :
+  'uuuuu .
+    'uuuuu ->
+      Prims.string ->
+        FStar_Compiler_Range_Type.range ->
+          (FStar_Parser_AST_Util.error_message,
+            FStar_Parser_AST.decl Prims.list) FStar_Pervasives.either
   =
-  fun s ->
-    fun r ->
-      FStar_Compiler_Util.print1 "Parsing somelang: <%s>\n" s;
-      (let uu___1 = FStar_Parser_ParseIt.parse_string_incrementally s in
-       match uu___1 with
-       | FStar_Pervasives.Inr (FStar_Pervasives_Native.None) ->
-           FStar_Compiler_Effect.failwith "Pulse parser failed"
-       | FStar_Pervasives.Inr (FStar_Pervasives_Native.Some (err, r1)) ->
-           FStar_Pervasives.Inl
-             {
-               FStar_Parser_AST_Util.message = err;
-               FStar_Parser_AST_Util.range = r1
-             }
-       | FStar_Pervasives.Inl (decls, first_error) ->
-           ((let uu___3 =
-               FStar_Class_Show.show
-                 (FStar_Class_Show.show_list FStar_Parser_AST.showable_decl)
-                 decls in
-             FStar_Compiler_Util.print1 "Parsed somelang decls: %s\n" uu___3);
-            FStar_Pervasives.Inr decls))
+  fun uu___ ->
+    fun s ->
+      fun r ->
+        FStar_Compiler_Util.print1 "Parsing somelang: <%s>\n" s;
+        (let uu___2 = FStar_Parser_ParseIt.parse_string_incrementally s in
+         match uu___2 with
+         | FStar_Pervasives.Inr (FStar_Pervasives_Native.None) ->
+             FStar_Compiler_Effect.failwith "Pulse parser failed"
+         | FStar_Pervasives.Inr (FStar_Pervasives_Native.Some (err, r1)) ->
+             FStar_Pervasives.Inl
+               {
+                 FStar_Parser_AST_Util.message = err;
+                 FStar_Parser_AST_Util.range = r1
+               }
+         | FStar_Pervasives.Inl (decls, first_error) ->
+             ((let uu___4 =
+                 FStar_Class_Show.show
+                   (FStar_Class_Show.show_list FStar_Parser_AST.showable_decl)
+                   decls in
+               FStar_Compiler_Util.print1 "Parsed somelang decls: %s\n"
+                 uu___4);
+              FStar_Pervasives.Inr decls))
 let (parse_incremental_decls_use_lang : unit -> unit) =
   fun uu___ ->
     let source0 =
