src/parser/FStar.Parser.AST.Util.fsti
@@ -59,11 +59,13 @@ val lookup_extension_parser (extension_name:string) : option extension_parser
 
 type extension_lang_parser = {
   parse_decls:
-   (contents:string ->
+   (option open_namespaces_and_abbreviations ->
+    contents:string ->
     p:FStar.Compiler.Range.range ->
     either error_message (list decl))
 }
 
+val as_open_namespaces_and_abbrevs (ls:list decl) : open_namespaces_and_abbreviations
 val register_extension_lang_parser (extension_name:string) (parser:extension_lang_parser) : unit
 val lookup_extension_lang_parser (extension_name:string) : option extension_lang_parser
-val parse_extension_lang (lang_name:string) (raw_text:string) (raw_text_pos:FStar.Compiler.Range.range) : list decl
+val parse_extension_lang (lang_name:string) (_:option open_namespaces_and_abbreviations) (raw_text:string) (raw_text_pos:FStar.Compiler.Range.range) : list decl
